ott_coq/destination_calculus_sugar_typing.v
@@ -16,8 +16,9 @@ Require Import Coq.Logic.ProofIrrelevance.
 Require Import Coq.Arith.Plus.
 Require Import Arith.
 Require Import Dest.destination_calculus_proofs.
+Require Import Lia.
 
-Theorem Ty_termS_Alloc : forall (P : ctx) (T : type), DisposableOnly P -> P ⊢ alloc : T ⧔ (⌊ T ⌋ ¹ν).
+Theorem Ty_term_termS_Alloc : forall (P : ctx) (T : type), DisposableOnly P -> P ⊢ alloc : T ⧔ (⌊ T ⌋ ¹ν).
 Proof.
   intros P T DisposP.
   unfold termS_Alloc.
@@ -42,7 +43,7 @@ Proof.
   - + apply DestOnly_empty.
 Qed.
 
-Theorem Ty_termS_FromA' : forall (P : ctx) (t : term) (T : type), P ⊢ t : T ⧔ ① -> P ⊢ from⧔' t : T.
+Theorem Ty_term_termS_FromA' : forall (P : ctx) (t : term) (T : type), P ⊢ t : T ⧔ ① -> P ⊢ from⧔' t : T.
 Proof.
   intros * Tyt.
   unfold termS_FromA'.
@@ -69,4 +70,130 @@ Proof.
     + rewrite union_commutative. apply Ty_term_PatU.
       * cbn. rewrite union_empty_l_eq at 1. apply Ty_term_Var. { apply DisposableOnly_empty. } { apply Disjoint_empty_l. } { repeat constructor. }
       * rewrite union_empty_l_eq with (G := ᴳ{ 1 : ¹ν ‗ T}). apply Ty_term_Var. { apply DisposableOnly_empty. }  { apply Disjoint_empty_l. } { repeat constructor. }
+Qed.
+
+Lemma Ty_term_termS_FillLeaf : forall (P1 P2 : ctx) (t t' : term) (T : type) (n : mode), IsValid n -> P1 ⊢ t : ⌊T⌋n -> P2 ⊢ t' : T -> P1 ᴳ+ (¹↑ · n) ᴳ·P2 ⊢ t ˢ⨞ t' : ①.
+Proof.
+  intros * Validn Tyt Tyt'.
+  unfold termS_FillLeaf.
+  replace (¹↑ · n) with (mode_times' ((¹↑ :: nil) ++ (n :: nil) ++ nil)). 2:{ cbn. destruct n; try destruct p; try destruct p2, a2; cbn; try destruct m, a; cbn; try rewrite Nat.add_0_r; trivial. }
+  apply Ty_term_FillC with (U := T); trivial.
+  apply Ty_term_ToA. assumption.
+Qed.
+
+Lemma Ty_term_termS_F : forall (P2 : ctx) (x: var) (m: mode) (u : term) (T U : type), UserDefined P2 -> IsValid m -> P2 # ᴳ{ x : m ‗ T} -> P2 ᴳ+ ᴳ{ x : m ‗ T} ⊢ u : U -> P2 ⊢ ˢλ x ⁔ m ⟼ u : T ⁔ m → U.
+Proof.
+  intros * UserDefinedP2 Validm DisjointP2x Tyu.
+  unfold termS_F.
+  apply Ty_term_termS_FromA'.
+  rewrite union_empty_l_eq with (G := P2).
+  apply Ty_term_Map with (T := ⌊T ⁔ m → U⌋ ¹ν).
+  { apply UserDefined_Disjoint; trivial. lia. }
+  apply Ty_term_termS_Alloc. apply DisposableOnly_empty.
+  rewrite union_commutative.
+  replace (¹↑) with (mode_times' ((¹↑ :: nil) ++ (¹ν :: nil) ++ nil)). 2:{ cbn. reflexivity. }
+  apply Ty_term_FillF with (T := T) (U := U); trivial.
+  constructor.
+  rewrite union_empty_l_eq with (G := ᴳ{ 0 : ¹ν ‗ ⌊ T ⁔ m → U ⌋ ¹ν}). apply Ty_term_Var. { apply DisposableOnly_empty. } { apply Disjoint_empty_l. } { repeat constructor. }
+Qed.
+
+Lemma Ty_term_termS_L : forall (P2 : ctx) (t : term) (T1 T2 : type), UserDefined P2 -> P2 ⊢ t : T1 -> P2 ⊢ ˢInl t : T1 ⨁ T2.
+Proof.
+  intros * UserDefinedP2 Tyt.
+  unfold termS_L.
+  apply Ty_term_termS_FromA'.
+  rewrite union_empty_l_eq with (G := P2).
+  apply Ty_term_Map with (T := ⌊T1 ⨁ T2⌋ ¹ν).
+  { apply UserDefined_Disjoint; trivial. lia. }
+  apply Ty_term_termS_Alloc. apply DisposableOnly_empty.
+  rewrite union_commutative.
+  replace (¹↑) with (¹↑ · ¹ν). 2:{ cbn. reflexivity. }
+  apply Ty_term_termS_FillLeaf with (T := T1); trivial.
+  constructor.
+  apply Ty_term_FillL with (T1 := T1) (T2 := T2); trivial.
+  rewrite union_empty_l_eq with (G := ᴳ{ 0 : ¹ν ‗ ⌊ T1 ⨁ T2 ⌋ ¹ν}). apply Ty_term_Var. { apply DisposableOnly_empty. } { apply Disjoint_empty_l. } { repeat constructor. }
+Qed.
+
+Lemma Ty_term_termS_R : forall (P2 : ctx) (t : term) (T1 T2 : type), UserDefined P2 -> P2 ⊢ t : T2 -> P2 ⊢ ˢInr t : T1 ⨁ T2.
+Proof.
+  intros * UserDefinedP2 Tyt.
+  unfold termS_R.
+  apply Ty_term_termS_FromA'.
+  rewrite union_empty_l_eq with (G := P2).
+  apply Ty_term_Map with (T := ⌊T1 ⨁ T2⌋ ¹ν).
+  { apply UserDefined_Disjoint; trivial. lia. }
+  apply Ty_term_termS_Alloc. apply DisposableOnly_empty.
+  rewrite union_commutative.
+  replace (¹↑) with (¹↑ · ¹ν). 2:{ cbn. reflexivity. }
+  apply Ty_term_termS_FillLeaf with (T := T2); trivial.
+  constructor.
+  apply Ty_term_FillR with (T1 := T1) (T2 := T2); trivial.
+  rewrite union_empty_l_eq with (G := ᴳ{ 0 : ¹ν ‗ ⌊ T1 ⨁ T2 ⌋ ¹ν}). apply Ty_term_Var. { apply DisposableOnly_empty. } { apply Disjoint_empty_l. } { repeat constructor. }
+Qed.
+
+Lemma Ty_term_termS_E : forall (P2 : ctx) (m : mode) (t : term) (T : type), UserDefined P2 -> IsValid m -> P2 ⊢ t : T -> m ᴳ· P2 ⊢ ˢᴇ m ⁔ t : ! m ⁔ T.
+Proof.
+  intros * UserDefinedP2 Validm Tyt.
+  unfold termS_E.
+  apply Ty_term_termS_FromA'.
+  rewrite union_empty_l_eq with (G := m ᴳ· P2).
+  apply Ty_term_Map with (T := ⌊! m ⁔ T⌋ ¹ν).
+  { apply UserDefined_Disjoint; trivial.
+    unfold UserDefined in *. intros x. specialize (UserDefinedP2 x). unfold stimes. rewrite In_map_iff. assumption.
+    lia. }
+  apply Ty_term_termS_Alloc. apply DisposableOnly_empty.
+  rewrite union_commutative.
+  rewrite stimes_is_action.
+  apply Ty_term_termS_FillLeaf with (P2 := P2) (T := T); trivial.
+  replace (⌊ T ⌋ m) with (⌊ T ⌋ mode_times' ((m :: nil) ++ (¹ν :: nil) ++ nil)). 2: { f_equal. cbn. apply mode_times_linnu_r_eq. }
+  apply Ty_term_FillE.
+  constructor.
+  rewrite union_empty_l_eq with (G := ᴳ{ 0 : ¹ν ‗ ⌊ ! m ⁔ T ⌋ ¹ν}). apply Ty_term_Var. { apply DisposableOnly_empty. } { apply Disjoint_empty_l. } { repeat constructor. }
+Qed.
+
+Lemma Ty_term_termS_P : forall (P21 P22 : ctx) (t1 t2 : term) (T1 T2 : type), UserDefined P21 -> UserDefined P22 -> P21 ⊢ t1 : T1 -> P22 ⊢ t2 : T2 -> (P21 ᴳ+ P22) ⊢ ˢ(t1, t2) : T1 ⨂ T2.
+Proof.
+  intros * UserDefinedP21 UserDefinedP22 Tyt1 Tyt2.
+  assert (UserDefined (P21 ᴳ+ P22)).
+  { apply UserDefined_union_iff. split; assumption. }
+  unfold termS_P.
+  apply Ty_term_termS_FromA'.
+  rewrite union_empty_l_eq with (G := P21 ᴳ+ P22).
+  apply Ty_term_Map with (T := ⌊T1 ⨂ T2⌋ ¹ν).
+  { apply UserDefined_Disjoint; trivial. lia. }
+  apply Ty_term_termS_Alloc. apply DisposableOnly_empty.
+  rewrite union_commutative.
+  replace (ᴳ{ 0 : ¹ν ‗ ⌊ T1 ⨂ T2 ⌋ ¹ν}) with (¹ν ᴳ· ᴳ{ 0 : ¹ν ‗ ⌊ T1 ⨂ T2 ⌋ ¹ν}). 2:{ rewrite stimes_linnu_eq. reflexivity. }
+  apply Ty_term_PatP with (T1 := ⌊ T1 ⌋ ¹ν) (T2 := ⌊ T2 ⌋ ¹ν).
+  constructor.
+  { apply UserDefined_Disjoint; trivial.
+    unfold UserDefined in *. intros x. specialize (H x). unfold stimes. rewrite In_map_iff. assumption.
+  unfold max_runtime_var. lia. } { apply UserDefined_Disjoint; trivial.
+    unfold UserDefined in *. intros x. specialize (H x). unfold stimes. rewrite In_map_iff. assumption.
+  unfold max_runtime_var. lia. }
+  apply Disjoint_singletons_iff. injection. inversion H0.
+  apply Ty_term_FillP with (T1 := T1) (T2 := T2); trivial.
+  rewrite union_empty_l_eq with (G := ᴳ{ 0 : ¹ν ‗ ⌊ T1 ⨂ T2 ⌋ ¹ν}). apply Ty_term_Var. { apply DisposableOnly_empty. } { apply Disjoint_empty_l. } { repeat constructor. }
+  replace (¹↑ ᴳ· (P21 ᴳ+ P22) ᴳ+ ᴳ{ 1 : ¹ν ‗ ⌊ T1 ⌋ ¹ν} ᴳ+ ᴳ{ 2 : ¹ν ‗ ⌊ T2 ⌋ ¹ν}) with ((ᴳ{ 1 : ¹ν ‗ ⌊ T1 ⌋ ¹ν} ᴳ+ ¹↑ ᴳ· P21) ᴳ+ (ᴳ{ 2 : ¹ν ‗ ⌊ T2 ⌋ ¹ν} ᴳ+ ¹↑ ᴳ· P22)). 2:{ rewrite stimes_distrib_on_union. rewrite union_commutative with (G1 := ᴳ{ 1 : ¹ν ‗ ⌊ T1 ⌋ ¹ν}). rewrite union_associative. rewrite <- union_associative with (G1 := ¹↑ ᴳ· P21). rewrite <- union_associative. rewrite union_commutative with (G1 := ᴳ{ 1 : ¹ν ‗ ⌊ T1 ⌋ ¹ν} ᴳ+ ᴳ{ 2 : ¹ν ‗ ⌊ T2 ⌋ ¹ν}). crush. }
+  apply Ty_term_PatU;
+  replace (¹↑) with (¹↑ · ¹ν); try (cbn; reflexivity).
+  apply Ty_term_termS_FillLeaf with (P2 := P21) (T := T1); trivial.
+  constructor.
+  rewrite union_empty_l_eq with (G := ᴳ{ 1 : ¹ν ‗ ⌊ T1 ⌋ ¹ν}). apply Ty_term_Var. { apply DisposableOnly_empty. } { apply Disjoint_empty_l. } { repeat constructor. }
+  apply Ty_term_termS_FillLeaf with (P2 := P22) (T := T2); trivial.
+  constructor.
+  rewrite union_empty_l_eq with (G := ᴳ{ 2 : ¹ν ‗ ⌊ T2 ⌋ ¹ν}). apply Ty_term_Var. { apply DisposableOnly_empty. } { apply Disjoint_empty_l. } { repeat constructor. }
+Qed.
+
+Theorem Ty_termS_coherency : forall (P : ctx) (t : term) (T : type), P ˢ⊢ t : T -> P ⊢ t : T.
+Proof.
+  intros * Tyst. inversion Tyst; subst. inversion Tyst; subst.
+  - apply Ty_term_termS_Alloc; trivial.
+  - apply Ty_term_termS_FromA'; trivial.
+  - replace (mode_times' ((¹↑ :: nil) ++ (n :: nil) ++ nil)) with (¹↑ · n). 2:{ cbn. destruct n; try destruct p; try destruct p2, a2; cbn; try destruct m, a; cbn; try rewrite Nat.add_0_r; trivial. } apply Ty_term_termS_FillLeaf with (T := T0); trivial.
+  - apply Ty_term_termS_F; trivial.
+  - apply Ty_term_termS_L; trivial.
+  - apply Ty_term_termS_R; trivial.
+  - apply Ty_term_termS_E; trivial.
+  - apply Ty_term_termS_P; trivial.
 Qed.
